Fix word_simp and proof

compiler/backend/word_simpScript.sml
@@ -320,7 +320,7 @@ val const_fp_loop_def = Define `
   (const_fp_loop (FFI x0 x1 x2 names) cs = (FFI x0 x1 x2 names, inter cs names)) /\
   (const_fp_loop (LocValue v x3) cs = (LocValue v x3, delete v cs)) /\
   (const_fp_loop (Alloc n names) cs = (Alloc n names, filter_v is_gc_const (inter cs names))) /\
-  (const_fp_loop (Install r1 r2 r3 r4 names) cs = (Install r1 r2 r3 r4 names, filter_v is_gc_const (inter cs names))) /\
+  (const_fp_loop (Install r1 r2 r3 r4 names) cs = (Install r1 r2 r3 r4 names, delete r1 (filter_v is_gc_const (inter cs names)))) /\
   (const_fp_loop p cs = (p, cs))`;
 
 val const_fp_loop_pmatch = Q.store_thm("const_fp_loop_pmatch",`!p cs.
@@ -360,7 +360,7 @@ val const_fp_loop_pmatch = Q.store_thm("const_fp_loop_pmatch",`!p cs.
   | (FFI x0 x1 x2 names) => (FFI x0 x1 x2 names, inter cs names)
   | (LocValue v x3) => (LocValue v x3, delete v cs)
   | (Alloc n names) => (Alloc n names, filter_v is_gc_const (inter cs names))
-  | (Install r1 r2 r3 r4 names) => (Install r1 r2 r3 r4 names, filter_v is_gc_const (inter cs names))
+  | (Install r1 r2 r3 r4 names) => (Install r1 r2 r3 r4 names, delete r1 (filter_v is_gc_const (inter cs names)))
   | p => (p, cs)`,
   rpt strip_tac
   >> CONV_TAC(patternMatchesLib.PMATCH_LIFT_BOOL_CONV true)
